examples/Sek/SWChunkOf.v
@@ -19,10 +19,10 @@ Require Import Owner_ml.
 Require Import Weighted_ml.
 Require Import SWChunk_ml.
 Require Import Capacity_proof.
+Require Import Weighted_proof.
 Require Import View_proof.
 Require Import SChunk_proof.
 Require Import SWChunk_proof.
-
 
 
 
@@ -40,13 +40,13 @@ Admitted.
 Notation "'Whtype' A a" := (htype (weighted_ A) (weighted_ a)) (at level 69, A at level 0).
 
 Definition SWChunkOf_MaybeOwned a A {IA: Inhab a} {EA: Enc a} (R: Whtype A a)
-	(M: SWChunkMem a) (oo: option owner_) (L: Wlist A) (s: swchunk_ a) : hprop :=
+	(M: SWChunkMem a) (oo: option owner_) (L: listW A) (s: swchunk_ a) : hprop :=
 	\exists l,
 		s ~> SWChunk_MaybeOwned M oo l \*
 		hfold_list2 R L l.
 
 Lemma SWChunkOf_MaybeOwned_eq : forall a (s: swchunk_ a) A (IA: Inhab a) (EA: Enc a) (R: Whtype A a)
-	(M: SWChunkMem a) (oo: option owner_) (L: Wlist A),
+	(M: SWChunkMem a) (oo: option owner_) (L: listW A),
 	s ~> SWChunkOf_MaybeOwned R M oo L = 
 		\exists l,
 			s ~> SWChunk_MaybeOwned M oo l \*
@@ -54,16 +54,21 @@ Lemma SWChunkOf_MaybeOwned_eq : forall a (s: swchunk_ a) A (IA: Inhab a) (EA: En
 Proof using. auto. Qed.
 
 Lemma SWChunkOf_MaybeOwned_Mono : forall a A {IA: Inhab a} {EA: Enc a} (R: Whtype A a)
-	(M M': SWChunkMem a) (oo: option owner_) (L: Wlist A) (c: swchunk_ a),
+	(M M': SWChunkMem a) (oo: option owner_) (L: listW A) (c: swchunk_ a),
 	SChunkExtend M M' ->
 	(c ~> SWChunkOf_MaybeOwned R M oo L ==> c ~> SWChunkOf_MaybeOwned R M' oo L).
+Admitted.
+
+Lemma SWChunkOf_MaybeOwned_inv_Inv : forall a A (IA: Inhab a) (EA: Enc a) (R: Whtype A a)
+	(M: SWChunkMem a) (oo: option owner_) (L: listW A) (c: swchunk_ a),
+	c ~> SWChunkOf_MaybeOwned R M oo L ==+> \[SWChunk_inv L (weight' c)].
 Admitted.
 
 (* ******************************************************* *)
 (** ** Specifications *)
 
 Lemma swchunk_default_spec_of : forall a A (IA: Inhab a) (EA: Enc a) (R: Whtype A a)
-	(M: SWChunkMem a) (oo: option owner_) (L: Wlist A) (c: swchunk_ a),
+	(M: SWChunkMem a) (oo: option owner_) (L: listW A) (c: swchunk_ a),
 	SPEC (swchunk_default c)
 		INV (c ~> SWChunkOf_MaybeOwned (a := a) (A := A) R M oo L)
 		POST (fun (d: a) => \[]).
@@ -76,13 +81,13 @@ Lemma swchunk_create_spec_of : forall a A (IA: Inhab a) (EA: Enc a) (R: Whtype A
 	SPEC (swchunk_create d oo)
 		MONO M
 		PRE \[]
-		POST (fun M' c => c ~> SWChunkOf_MaybeOwned (a := a) (A := A) R M' oo (@nil (weighted_ A))).
+		POST (fun M' c => c ~> SWChunkOf_MaybeOwned R M' oo nil).
 Admitted.
 
 Hint Extern 1 (RegisterSpec swchunk_create) => Provide swchunk_create_spec_of.
 
 Lemma swchunk_is_full_spec_of : forall a A (IA: Inhab a) (EA: Enc a) (R: Whtype A a)
-	(M: SWChunkMem a) (oo: option owner_) (L: Wlist A) (c: swchunk_ a),
+	(M: SWChunkMem a) (oo: option owner_) (L: listW A) (c: swchunk_ a),
 	SPEC (swchunk_is_full c)
 		INV (c ~> SWChunkOf_MaybeOwned R M oo L)
 		POST (fun b => \[b = isTrue (IsFull L)]).
@@ -91,7 +96,7 @@ Proof using. skip. Qed.
 Hint Extern 1 (RegisterSpec swchunk_is_full) => Provide swchunk_is_full_spec_of.
 
 Lemma swchunk_push_spec_of : forall a A (IA: Inhab a) (EA: Enc a) (R: Whtype A a)
-	(v: view_) (M: SWChunkMem a) (oo: option owner_) (L: Wlist A) (c: swchunk_ a) (X: weighted_ A) (x: weighted_ a),
+	(v: view_) (M: SWChunkMem a) (oo: option owner_) (L: listW A) (c: swchunk_ a) (X: weighted_ A) (x: weighted_ a),
 	SPEC (swchunk_push v oo c x)
 	MONO M
 	PRE (c ~> SWChunkOf_MaybeOwned R M oo L \* x ~> R X)
