examples/Sek/SWChunk_proof.v
@@ -29,11 +29,8 @@ Require Import SChunk_proof.
 (* ******************************************************* *)
 (** ** Representation predicates *)
 
-Definition list_sum A (W: A -> int) (L: list A) : int :=
-  LibList.fold_left (fun x acc => acc + W x) 0 L.
-
 Notation "'SWChunkMem' A" := (SChunkMem (weighted_ A)) (at level 69).
-Notation "'Wlist' A" := (list (weighted_ A)) (at level 69).
+
 
 Record SWChunk_inv A (L: list (weighted_ A)) (w: int) : Prop :=
 	mkSWChunk_inv {
@@ -43,29 +40,29 @@ Record SWChunk_inv A (L: list (weighted_ A)) (w: int) : Prop :=
 Definition SWChunk_IsOwner A {IA: Inhab A} {EA: Enc A} (oo: option owner_) (s: swchunk_ A) : Prop :=
 	SChunk_IsOwner oo (unweighted' s).
 
-(* Definition SWChunk_Shared A {IA: Inhab A} {EA: Enc A} (M: WChunkMemory A) (L: Wlist A) (s: swchunk_ A) : Prop :=
+(* Definition SWChunk_Shared A {IA: Inhab A} {EA: Enc A} (M: WChunkMemory A) (L: listW A) (s: swchunk_ A) : Prop :=
 	let '(c, w) := s in
 	SChunk_Shared M L c /\
 	SWChunk_inv L w.
 
-Definition SWChunk_UniquelyOwned A {IA: Inhab A} {EA: Enc A} (L: Wlist A) (s: swchunk_ A) : hprop :=
+Definition SWChunk_UniquelyOwned A {IA: Inhab A} {EA: Enc A} (L: listW A) (s: swchunk_ A) : hprop :=
 	let '(c, w) := s in
 	c ~> SChunk_UniquelyOwned L \*
 	\[SWChunk_inv L w].
 
-Definition SWChunk_MaybeOwned A {IA: Inhab A} {EA: Enc A}	(M: WChunkMemory A) (oo: option owner_) (L: Wlist A) (s: swchunk_ A) : hprop :=
+Definition SWChunk_MaybeOwned A {IA: Inhab A} {EA: Enc A}	(M: WChunkMemory A) (oo: option owner_) (L: listW A) (s: swchunk_ A) : hprop :=
 	If SWChunk_IsOwner oo s then
 		s ~> SWChunk_UniquelyOwned L
 	else
 		\[SWChunk_Shared M L s]. *)
 
-Definition SWChunk_MaybeOwned A {IA: Inhab A} {EA: Enc A}	(M: SWChunkMem A) (oo: option owner_) (L: Wlist A) (s: swchunk_ A) : hprop :=
+Definition SWChunk_MaybeOwned A {IA: Inhab A} {EA: Enc A}	(M: SWChunkMem A) (oo: option owner_) (L: listW A) (s: swchunk_ A) : hprop :=
 	let (c, w) := s in
 	c ~> SChunk_MaybeOwned M oo L \*
 	\[SWChunk_inv L w].
 
 Lemma SWChunk_MaybeOwned_Mono : forall A {IA: Inhab A} {EA: Enc A}
-	(M M': SWChunkMem A) (oo: option owner_) (L: Wlist A) (c: swchunk_ A),
+	(M M': SWChunkMem A) (oo: option owner_) (L: listW A) (c: swchunk_ A),
 	SChunkExtend M M' ->
 	(c ~> SWChunk_MaybeOwned M oo L ==> c ~> SWChunk_MaybeOwned M' oo L).
 Admitted.
@@ -82,11 +79,16 @@ Proof using. intros. apply weighted_inhab. apply~ partial_swchunk_inhab. Qed.
 Hint Resolve partial_swchunk_inhab swchunk_inhab.
 
 
+Lemma SWChunk_MaybeOwned_inv_Inv : forall A (IA: Inhab A) (EA: Enc A) (M: SWChunkMem A) (oo: option owner_) (L: listW A) (c: swchunk_ A),
+	c ~> SWChunk_MaybeOwned M oo L ==+> \[SWChunk_inv L (weight' c)].
+Admitted.
+
+
 (* ******************************************************* *)
 (** ** Specifications *)
 
 Lemma swchunk_push_spec : forall A (IA: Inhab A) (EA: Enc A)
-	(v: view_) (M: SWChunkMem A) (oo: option owner_) (L: Wlist A) (c: swchunk_ A) (x: weighted_ A),
+	(v: view_) (M: SWChunkMem A) (oo: option owner_) (L: listW A) (c: swchunk_ A) (x: weighted_ A),
 	SPEC (swchunk_push v oo c x)
 	MONO M
 	PRE (c ~> SWChunk_MaybeOwned M oo L)
